Managed to define 'related'

TypeSoundness.v
@@ -1,7 +1,5 @@
 (* Type soundness *)
 
-Set Implicit Arguments.
-
 Require Import List.
 Require Import Typing EvalCBV.
 
@@ -121,6 +119,55 @@ Definition sound_wrt_bounded :=
           ~ exists n e',
               nsteps (Eapp f v) n e' /\ n > C * n'.
 
+Require Import Util.
+Local Open Scope prog_scope.
+
+Inductive stepex : expr -> bool -> expr -> Prop :=
+| STecontext c e1 b e2 : stepex e1 b e2 -> stepex (plug c e1) b (plug c e2)
+| STapp t body arg : IsValue arg -> stepex (Eapp (Eabs t body) arg) false (subst arg body)
+| STlet t v main : IsValue v -> stepex (Elet t v main) false (subst v main)
+| STmatch_pair ta tb a b k : 
+    IsValue a ->
+    IsValue b ->
+    stepex (Ematch_pair (Epair $$ ta $$ tb $$ a $$ b) k) false (subst_list [a; b] k)
+| STmatch_inl ta tb v k1 k2 : 
+    IsValue v ->
+    stepex (Ematch_sum (Einl $$ ta $$ tb $$ v) k1 k2) false (subst v k1)
+| STmatch_inr ta tb v k1 k2 : 
+    IsValue v ->
+    stepex (Ematch_sum (Einr $$ ta $$ tb $$ v) k1 k2) false (subst v k2)
+| STtapp body t : stepex (Etapp (Etabs body) t) false (subst t body)
+| STunfold_fold v t1 : 
+    IsValue v ->
+    stepex (Eunfold (Efold t1 v)) true v
+| STunhide_hide v :
+    IsValue v ->
+    stepex (Eunhide (Ehide v)) false v
+.
+
+Inductive nstepsex : expr -> nat -> nat -> expr -> Prop :=
+| NEsteps0 e : nstepsex e 0 0 e
+| NEstepsS e1 b e2 n m e3 : stepex e1 b e2 -> nstepsex e2 n m e3 -> nstepsex e1 (S n) ((if b then 1 else 0) + m) e3
+.
+
+Class Leb A B :=
+  {
+    leb : A -> B -> bool
+  }.
+
+Infix "<=?" := leb (at level 70).
+
+Definition lebCS : csize -> csize -> bool.
+  admit.
+Defined.
+
+Instance Leb_csize_csize : Leb csize csize :=
+  {
+    leb := lebCS
+  }.
+
+Definition cexpr_to_nat (c : cexpr) := default 0 (nat_of_cexpr c).
+
 (* A Parametric Higher-Order Abstract Syntax (PHOAS) encoding for a second-order modal logic (LSLR) *)
 
 Section rel.
@@ -148,170 +195,6 @@ Section rel.
   .
 
 End rel.
-
-Module ClosedPHOAS.
-
-Notation "⊤" := (Rtrue _).
-Notation "⊥" := (Rtrue _).
-(* Notation "\ e , p" := (Rabs (fun e => p)) (at level 200, format "\ e , p"). *)
-Notation "\ x .. y , p" := (Rabs (fun x => .. (Rabs (fun y => p)) ..)) (at level 200, x binder, y binder, right associativity).
-Notation "∀ x .. y , p" := (Rforalle (fun x => .. (Rforalle (fun y => p)) ..)) (at level 200, x binder, y binder, right associativity).
-Notation "∃ x .. y , p" := (Rexistse (fun x => .. (Rexistse (fun y => p)) ..)) (at level 200, x binder, y binder, right associativity).
-Notation "∀1 x .. y , p" := (Rforall1 (fun x => .. (Rforall1 (fun y => p)) ..)) (at level 200, x binder, y binder, right associativity).
-Notation "∃1 x .. y , p" := (Rexists1 (fun x => .. (Rexists1 (fun y => p)) ..)) (at level 200, x binder, y binder, right associativity).
-Definition RforallR' var n P := (@RforallR var n (fun x => P (Rvar _ _ x))).
-Notation "∀2 x .. y , p" := (RforallR' (fun x => .. (RforallR' (fun y => p)) ..)) (at level 200, x binder, y binder, right associativity).
-Definition RexistsR' var n P := (@RexistsR var n (fun x => P (Rvar _ _ x))).
-Notation "∃2 x .. y , p" := (RexistsR' (fun x => .. (RexistsR' (fun y => p)) ..)) (at level 200, x binder, y binder, right associativity).
-Definition Rrecur' var n P := (@Rrecur var n (fun x => P (Rvar _ _ x))).
-Notation "@ x .. y , p" := (Rrecur' (fun x => .. (Rrecur' (fun y => p)) ..)) (at level 200, x binder, y binder, right associativity).
-Notation "⌈ P ⌉" := (Rinj _ P).
-Notation "e ∈ P" := (Rapp P e) (at level 70).
-Infix "/\" := Rand.
-Infix "\/" := Ror.
-Infix "⇒" := Rimply (at level 90).
-Notation "▹" := Rlater.
-Definition VSet var τ (S : rel var 1) := ∀ v, v ∈ S ⇒ ⌈v ↓ τ⌉.
-
-Section TestNotations.
-  
-  Variable var : nat -> Type.
-
-  Definition ttt1 : rel var 1 := \e , ⊤.
-  Definition ttt2 : rel var 1 := \e , ⌈e ↓ Tunit⌉.
-  Definition ttt3 : rel var 1 := \_ , ⌈True /\ True⌉.
-
-End TestNotations.
-
-Inductive thresholds :=
-| THleaf
-| THarrow : thresholds -> csize -> thresholds -> thresholds
-.
-
-Require Import Util.
-Local Open Scope prog_scope.
-
-(* A "step-indexed" kriple model *)
-
-(* the logical relation *)
-Section LR.
-  
-  Variable var : nat -> Type.
-
-  Definition substs : Type.
-    admit.
-  Defined.
-
-  Definition substs_type : substs -> type -> type.
-    admit.
-  Defined.
-
-  Coercion substs_type : substs >-> Funclass.
-
-  Definition substs_sem : substs -> nat -> rel var 1.
-    admit.
-  Defined.
-
-  Instance Apply_substs_nat_rel : Apply substs nat (rel var 1) :=
-    {
-      apply := substs_sem
-    }.
-
-  Definition substs_cexpr : substs -> cexpr -> cexpr.
-    admit.
-  Defined.
-
-  Instance Apply_substs_cexpr_cexpr : Apply substs cexpr cexpr :=
-    {
-      apply := substs_cexpr
-    }.
-
-  Definition substs_size : substs -> size -> size.
-    admit.
-  Defined.
-
-  Instance Apply_substs_size_size : Apply substs size size :=
-    {
-      apply := substs_size
-    }.
-
-  Definition add_csize : csize -> substs -> substs.
-    admit.
-  Defined.
-
-  Instance Add_csize_substs : Add csize substs substs :=
-    {
-      add := add_csize
-    }.
-
-  Definition add_pair : (type * rel var 1) -> substs -> substs.
-    admit.
-  Defined.
-
-  Instance Add_pair_substs : Add (type * rel var 1) substs substs :=
-    {
-      add := add_pair
-    }.
-
-  Inductive stepex : expr -> bool -> expr -> Prop :=
-  | STecontext c e1 b e2 : stepex e1 b e2 -> stepex (plug c e1) b (plug c e2)
-  | STapp t body arg : IsValue arg -> stepex (Eapp (Eabs t body) arg) false (subst arg body)
-  | STlet t v main : IsValue v -> stepex (Elet t v main) false (subst v main)
-  | STmatch_pair ta tb a b k : 
-      IsValue a ->
-      IsValue b ->
-      stepex (Ematch_pair (Epair $$ ta $$ tb $$ a $$ b) k) false (subst_list [a; b] k)
-  | STmatch_inl ta tb v k1 k2 : 
-      IsValue v ->
-      stepex (Ematch_sum (Einl $$ ta $$ tb $$ v) k1 k2) false (subst v k1)
-  | STmatch_inr ta tb v k1 k2 : 
-      IsValue v ->
-      stepex (Ematch_sum (Einr $$ ta $$ tb $$ v) k1 k2) false (subst v k2)
-  | STtapp body t : stepex (Etapp (Etabs body) t) false (subst t body)
-  | STunfold_fold v t1 : 
-      IsValue v ->
-      stepex (Eunfold (Efold t1 v)) true v
-  | STunhide_hide v :
-      IsValue v ->
-      stepex (Eunhide (Ehide v)) false v
-  .
-
-  Inductive nstepsex : expr -> nat -> nat -> expr -> Prop :=
-  | NEsteps0 e : nstepsex e 0 0 e
-  | NEstepsS e1 b e2 n m e3 : stepex e1 b e2 -> nstepsex e2 n m e3 -> nstepsex e1 (S n) ((if b then 1 else 0) + m) e3
-  .
-
-  Program Fixpoint E' V τ (n : nat) (s : size) (ρ : substs) (C : nat) (θ : thresholds) {measure n} : rel var 1 :=
-    \e, ⌈|~ [] e (ρ τ)⌉ /\ 
-        ∀1 n', ∀ e', 
-          (⌈nstepsex e n' 0 e'⌉ ⇒ ⌈n' ≤ n⌉ /\ (⌈IsValue e'⌉ ⇒ e' ∈ V τ ρ C θ /\ ⌈|e'| ≤ s⌉)) /\
-          match n with
-            | 0 => ⊤
-            | S _ =>
-              (⌈nstepsex e (S n') 1 e'⌉ ⇒ ⌈(S n') ≤ n⌉ /\ ▹ (e' ∈ E' V τ (n - S n') s ρ C θ))
-          end.
-  Next Obligation.
-    omega.
-  Defined.
-
-  Fixpoint V τ (ρ : substs) (C : nat) (θ : thresholds) {struct τ} : rel var 1 :=
-    match τ, θ with
-      | Tvar α, _ => ρ $ α
-      | Tunit, _ => \v, ⌈v ↓ τ⌉
-      | τ₁ × τ₂, _ => \v, ⌈v ↓ ρ τ⌉ /\ ∃ a b, ⌈v = Epair a b⌉ /\ a ∈ V τ₁ ρ C θ /\ b ∈ V τ₂ ρ C θ
-      | τ₁ + τ₂, _ => \v, ⌈v ↓ ρ τ⌉ /\ ∃ v', (⌈v = Einl τ₂ v'⌉ /\ v' ∈ V τ₁ ρ C θ) ‌\/ ⌈v = Einr τ₁ v'⌉ /\ v' ∈ V τ₂ ρ C θ
-      | Tarrow τ₁ c s τ₂, _, THarrow θ₁ ξ₀ θ₂ => \v, ⌈v ↓ ρ τ⌉ /\ ∀ v₁, v₁ ∈ V τ₁ ρ C θ /\ ⌈ξ₀ ≤ |v₁|⌉ ⇒ Eapp v v₁ ∈ E' V τ₂ c s (add ξ₁ ρ) C θ₂
-      | Tuniversal c s τ, _ => \v, ⌈v ↓ ρ τ⌉ /\ ∀1 τ', ∀2 S, VSet τ' S ⇒ Etapp v τ' ∈ E' V τ c s (add (τ', S) ρ) C θ
-      | Trecur τ, _ => @S, \v, ⌈v ↓ ρ τ⌉ /\ ∃ v', ⌈v = Efold τ v'⌉ /\ ▹ (v' ∈ V τ (add (ρ τ, S) ρ) C θ)
-      | _, _, _ => \_, ⊥
-    end
-  .
-
-  Definition E := E' V.
-
-End LR.
-
-End ClosedPHOAS.
 
 Module OpenPHOAS.
 
@@ -342,7 +225,7 @@ Section relOpen.
       | domain :: C' => interp domain -> relOpen C' range
     end.
 
-  Program Fixpoint liftToOpen C n1 n2 (f : rel var n1 -> rel var n2) (a : relOpen C n1) : relOpen C n2 :=
+  Program Fixpoint liftToOpen C {n1 n2} (f : rel var n1 -> rel var n2) (a : relOpen C n1) : relOpen C n2 :=
     match C with
       | nil => _
       | nv :: C' => _ (@liftToOpen C' n1 n2)
@@ -356,7 +239,7 @@ Section relOpen.
 
   Require Import Program.
 
-  Program Fixpoint liftToOpen2 C n1 n2 T (f : (T -> rel var n1) -> rel var n2) (a : T -> relOpen C n1) : relOpen C n2 :=
+  Program Fixpoint liftToOpen2 C {n1 n2 T} (f : (T -> rel var n1) -> rel var n2) (a : T -> relOpen C n1) : relOpen C n2 :=
     match C with
       | nil => _
       | nv :: C' => _ (@liftToOpen2 C' n1 n2)
@@ -368,19 +251,19 @@ Section relOpen.
     exact (x _ f (flip a X)).
   Defined.
 
-  Program Fixpoint liftToOpen3 C n T (f : T -> rel var n) (a : T) : relOpen C n :=
+  Program Fixpoint liftToOpen3 C {n T} (f : T -> rel var n) (a : T) : relOpen C n :=
     match C with
       | nil => _
       | nv :: C' => _ (@liftToOpen3 C' n)
     end.
 
-  Program Fixpoint liftToOpen4 C n (f : rel var n) : relOpen C n :=
+  Program Fixpoint liftToOpen4 C {n} (f : rel var n) : relOpen C n :=
     match C with
       | nil => _
       | nv :: C' => _ (@liftToOpen4 C' n)
     end.
 
-  Program Fixpoint liftToOpen5 C n1 n2 n3 (f : rel var n1 -> rel var n2 -> rel var n3) (a : relOpen C n1) (b : relOpen C n2) : relOpen C n3 :=
+  Program Fixpoint liftToOpen5 C {n1 n2 n3} (f : rel var n1 -> rel var n2 -> rel var n3) (a : relOpen C n1) (b : relOpen C n2) : relOpen C n3 :=
     match C with
       | nil => _
       | nv :: C' => _ (@liftToOpen5 C' n1 n2 n3)
@@ -392,7 +275,7 @@ Section relOpen.
     exact (x f (a X) (b X)).
   Defined.
 
-  Program Fixpoint liftToOpen6 C n1 T n2 (f : rel var n1 -> T -> rel var n2) (a : relOpen C n1) (b : T) : relOpen C n2 :=
+  Program Fixpoint liftToOpen6 C {n1 T n2} (f : rel var n1 -> T -> rel var n2) (a : relOpen C n1) (b : T) : relOpen C n2 :=
     match C with
       | nil => _
       | nv :: C' => _ (@liftToOpen6 C' n1 T n2)
@@ -486,11 +369,11 @@ Local Open Scope prog_scope.
 Section LR.
   
   Variable var : nat -> Type.
-  Variable C : Ctx.
+  Variable ctx : Ctx.
 
   Inductive SubstEntry :=
-  | SEtype (_ : relOpen var C (TTother type)) (_ : option (relOpen var C 1))
-  | SEexpr (_ : relOpen var C TTexpr) (_ : relOpen var C (TTother csize))
+  | SEtype (_ : relOpen var ctx (TTother type)) (_ : option (relOpen var ctx 1))
+  | SEexpr (_ : relOpen var ctx TTexpr) (_ : relOpen var ctx (TTother csize))
   .
 
   Definition substs : Type := list SubstEntry.
@@ -501,11 +384,345 @@ Section LR.
 
   Coercion substs_type : substs >-> Funclass.
 
-  Definition substs_sem : substs -> nat -> relOpen var C 1.
+  Definition substs_sem : substs -> nat -> relOpen var ctx 1.
     admit.
   Defined.
 
-  Instance Apply_substs_nat_rel : Apply substs nat (relOpen var C 1) :=
+  Instance Apply_substs_nat_rel : Apply substs nat (relOpen var ctx 1) :=
+    {
+      apply := substs_sem
+    }.
+
+  Definition substs_cexpr : substs -> cexpr -> cexpr.
+    admit.
+  Defined.
+
+  Instance Apply_substs_cexpr_cexpr : Apply substs cexpr cexpr :=
+    {
+      apply := substs_cexpr
+    }.
+
+  Definition substs_size : substs -> size -> size.
+    admit.
+  Defined.
+
+  Instance Apply_substs_size_size : Apply substs size size :=
+    {
+      apply := substs_size
+    }.
+
+  Definition substs_expr : substs -> expr -> expr.
+    admit.
+  Defined.
+
+  Instance Apply_substs_expr_expr : Apply substs expr expr :=
+    {
+      apply := substs_expr
+    }.
+
+  Definition add_csize : csize -> substs -> substs.
+    admit.
+  Defined.
+
+  Instance Add_csize_substs : Add csize substs substs :=
+    {
+      add := add_csize
+    }.
+
+  Definition add_pair : (type * relOpen var ctx 1) -> substs -> substs.
+    admit.
+  Defined.
+
+  Instance Add_pair_substs : Add (type * relOpen var ctx 1) substs substs :=
+    {
+      add := add_pair
+    }.
+
+  Program Fixpoint E' V τ (n : nat) (s : size) (ρ : substs) (Ct : nat) (θ : thresholds) {measure n} : relOpen var ctx 1 :=
+    \e, ⌈|~ [] e (ρ τ)⌉ /\ 
+        ∀1 n', ∀ e', 
+          (⌈nstepsex e n' 0 e'⌉ ⇒ ⌈n' ≤ n⌉ /\ (⌈IsValue e'⌉ ⇒ e' ∈ V ρ Ct θ /\ ⌈|e'| ≤ s⌉)) /\
+          match n with
+            | 0 => ⊤
+            | S _ =>
+              (⌈nstepsex e (S n') 1 e'⌉ ⇒ ⌈(S n') ≤ n⌉ /\ ▹ (e' ∈ E' V τ (n - S n') s ρ Ct θ))
+          end.
+  Next Obligation.
+    omega.
+  Defined.
+
+  Fixpoint V τ (ρ : substs) (Ct : nat) (θ : thresholds) {struct τ} : relOpen var ctx 1 :=
+    match τ, θ with
+      | Tvar α, _ => ρ $ α
+      | Tunit, _ => \v, ⌈v ↓ τ⌉
+      | τ₁ × τ₂, _ => \v, ⌈v ↓ ρ τ⌉ /\ ∃ a b, ⌈v = Epair a b⌉ /\ a ∈ V τ₁ ρ Ct θ /\ b ∈ V τ₂ ρ Ct θ
+      | τ₁ + τ₂, _ => \v, ⌈v ↓ ρ τ⌉ /\ ∃ v', (⌈v = Einl τ₂ v'⌉ /\ v' ∈ V τ₁ ρ Ct θ) /\ ⌈v = Einr τ₁ v'⌉ /\ v' ∈ V τ₂ ρ Ct θ
+      | Tarrow τ₁ c s τ₂, THarrow θ₁ ξ₀ θ₂ => \v, ⌈v ↓ ρ τ⌉ /\ ∀ v₁, v₁ ∈ V τ₁ ρ Ct θ ⇒ Eapp v v₁ ∈ E' (V τ₂) τ₂ (cexpr_to_nat c) s (add (if ξ₀ <=? |v₁| then |v₁| else ξ₀) ρ) Ct θ₂
+      | Tuniversal c s τ, _ => \v, ⌈v ↓ ρ τ⌉ /\ ∀1 τ', ∀2 S, VSet τ' S ⇒ Etapp v τ' ∈ E' (V τ) τ (cexpr_to_nat c) s (add (τ', S) ρ) Ct θ
+      | Trecur τ, _ => @S, \v, ⌈v ↓ ρ τ⌉ /\ ∃ v', ⌈v = Efold τ v'⌉ /\ ▹ (v' ∈ V τ (add (ρ τ, S) ρ) Ct θ)
+      | _, _ => \_, ⊥
+    end
+  .
+
+  Definition E τ := E' (V τ) τ.
+
+End LR.
+
+End OpenPHOAS.
+
+Import OpenPHOAS.
+
+Unset Strict Implicit.
+Unset Printing Implicit Defensive. 
+Generalizable All Variables.
+
+Section related.
+
+  Variable var : nat -> Type.
+
+  Class Lift A B :=
+    {
+      lift : forall (t : termType), A -> B t
+    }.
+
+  Instance Lift_list `{Lift A B} : Lift (list A) (fun t => list (B t)) :=
+    {
+      lift t a := map (lift t) a
+    }.
+
+  Definition lift_relOpen {ctx range} new : relOpen var ctx range -> relOpen var (new :: ctx) range.
+    admit.
+  Defined.
+
+  Instance Lift_relOpen ctx range : Lift (relOpen var ctx range) (fun new => relOpen var (new :: ctx) range) :=
+    {
+      lift := lift_relOpen
+    }.
+
+  Definition lift_SubstEntry {ctx} new : SubstEntry var ctx -> SubstEntry var (new :: ctx).
+    admit.
+  Defined.
+
+  Instance Lift_SubstEntry ctx : Lift (SubstEntry var ctx) (fun new => SubstEntry var (new :: ctx)) :=
+    {
+      lift := lift_SubstEntry
+    }.
+
+  Definition t_Ps_ρ ctx := (list (relOpen var ctx 0) * substs var ctx)%type.
+
+  Definition lift_Ps_ρ {ctx} t (Ps_ρ : t_Ps_ρ ctx) : t_Ps_ρ (t :: ctx):=
+    let (Ps, ρ) := Ps_ρ in
+    let Ps := map (lift_relOpen t) Ps in
+    let ρ := map (lift t) ρ in
+    (Ps, ρ).
+
+  Instance Lift_Ps_ρ ctx : Lift (t_Ps_ρ ctx) (fun new => t_Ps_ρ (new :: ctx))%type :=
+    {
+      lift := lift_Ps_ρ
+    }.
+
+  Definition extend {range} ctx new : relOpen var ctx range -> relOpen var (ctx ++ new) range.
+    admit.
+  Defined.
+
+  Notation TTtype := (TTother type).
+  Notation TTcsize := (TTother csize).
+
+  Arguments SEtype {var ctx} _ _ .
+  Arguments SEexpr {var ctx} _ _ .
+
+  Definition add_type {ctx} k (Ps_ρ : t_Ps_ρ ctx) : t_Ps_ρ (TTrel 1 :: TTtype :: ctx) :=
+    let (Ps, ρ) := lift_Ps_ρ TTtype Ps_ρ in
+    let Ps := extend [TTtype] ctx (fun τ => ⌈kinding [] τ k⌉ : relOpen var [] 0) :: Ps in
+    let (Ps, ρ) := lift_Ps_ρ 1 (Ps, ρ) in
+    match k with
+      | 0 => 
+        let Ps := extend [TTrel 1; TTtype] ctx (fun S τ => VSet τ (S : relOpen var [] 1)) :: Ps in
+        let ρ := SEtype (extend [TTrel 1; TTtype] ctx (fun _ τ => τ)) (Some (extend [TTrel 1; TTtype] ctx (fun S _ => S))) :: ρ in
+        (Ps, ρ)
+      | _ =>
+        let ρ := SEtype (extend [TTrel 1; TTtype] ctx (fun _ τ => τ)) None :: ρ in
+        (Ps, ρ)
+    end.
+
+  Arguments V {var ctx} _ _ _ _ .
+  Arguments E {var ctx} _ _ _ _ _ _ .
+
+  Definition csize_of_size : size -> option csize.
+    admit.
+  Defined.
+
+  Definition asCsize P s :=
+    (exists x, csize_of_size s = Some x /\ P x)%type.
+
+  Existing Instance Apply_substs_size_size.
+  Existing Instance Apply_substs_cexpr_cexpr.
+  Existing Instance Apply_substs_expr_expr.
+
+  Definition add_expr {ctx} τ θ (os : csize + size) Ct (Ps_ρ : t_Ps_ρ ctx) : t_Ps_ρ (TTcsize :: TTexpr :: ctx) :=
+    let (Ps, ρ) := Ps_ρ in
+    let ρ0 := ρ in
+    let (Ps, ρ) := lift_Ps_ρ TTexpr (Ps, ρ) in
+    let Ps := ((fun e => e ∈ V τ ρ0 Ct θ) : relOpen var (TTexpr :: ctx) 0) :: Ps in
+    let (Ps, ρ) := lift_Ps_ρ TTcsize (Ps, ρ) in
+    let ρ := SEexpr (extend [TTcsize; TTexpr] ctx (fun _ e => e)) (extend [TTcsize; TTexpr] ctx (fun ξ _ => ξ)) :: ρ in
+    match os with
+      | inl ξ₀ =>
+        let Ps := extend [TTcsize; TTexpr] ctx (fun ξ v => ⌈ξ = if ξ₀ <=? |v| then |v| else ξ₀⌉ : relOpen var [] 0) :: Ps in
+        (Ps, ρ)
+      | inr s =>
+        let Ps := extend [TTcsize; TTexpr] ctx (fun ξ _ => ⌈asCsize (fun ξ' => ξ = ξ') (ρ $$ s)⌉ : relOpen var [] 0) :: Ps in
+        (Ps, ρ)
+    end.
+
+  Inductive tc_entryex :=
+  | TEkindingex (_ : kind)
+  | TEtypingex (_ : type * thresholds * (csize + size))
+  .
+
+  Definition tcontextex := list tc_entryex.
+
+  Fixpoint make_ctx Γ :=
+    match Γ with
+      | nil => nil
+      | TEkindingex _ :: Γ' =>
+        TTrel 1 :: TTtype :: make_ctx Γ'
+      | TEtypingex _ :: Γ' =>
+        TTcsize :: TTexpr :: make_ctx Γ'
+    end.
+
+  Fixpoint make_Ps_ρ Γ Ct : t_Ps_ρ (make_ctx Γ) :=
+    match Γ return t_Ps_ρ (make_ctx Γ) with 
+      | nil => (nil, nil)
+      | TEkindingex k :: Γ' =>
+        let Ps_ρ := make_Ps_ρ Γ' Ct in
+        add_type k Ps_ρ
+      | TEtypingex (τ, θ, os) :: Γ' =>
+        let Ps_ρ := make_Ps_ρ Γ' Ct in
+        add_expr τ θ os Ct Ps_ρ
+    end.
+
+  Definition extendΓ : tcontext -> list csize -> list thresholds -> option tcontextex.
+    admit.
+  Defined.
+
+  Definition valid {ctx} (Ps : list (relOpen var ctx 0)) (P : relOpen var ctx 0) : Prop.
+    admit.
+  Defined.
+  Notation "Ps |- P" := (valid Ps P) (at level 90).
+
+  Definition related Γ (e : expr) τ (c : cexpr) (s : size) :=
+    (exists Ct ξs θs θ Γ',
+       extendΓ Γ ξs θs = Some Γ' /\
+       let (Ps, ρ) := make_Ps_ρ Γ' Ct in
+       Ps |- (ρ $ e) ∈ E τ (Ct * cexpr_to_nat (ρ $ c))%nat (ρ $ s) ρ Ct θ)%type.
+
+  Notation "⊩" := related.
+
+  Lemma foundamental :
+    forall Γ e τ c s,
+      ⊢ Γ e τ c s -> 
+      ⊩ Γ e τ c s.
+  Proof.
+    (* induction 1. *)
+    admit.
+  Qed.
+
+End related.
+      
+(*
+Section inferRules.
+
+  Variable var : nat -> Type.
+
+  Variable C : list nat.
+
+  Reserved Notation "C |- P" (at level 90).
+  
+  Inductive valid : list (relOpen var C 0) -> relOpen var C 0 -> Prop :=
+  | RuleMono C P : C |- P -> C |- ▹P
+  | RuleLob C P : ▹P :: C |- P -> C |- P
+  | RuleLaterAnd1 C P Q : C |- ▹ (P /\ Q) -> C |- ▹P /\ ▹Q
+  | RuleLaterAnd2 C P Q : C |- ▹P /\ ▹Q -> C |- ▹ (P /\ Q)
+  | RuleElem1 C P e : C |- e ∈ ORabs P -> C |- P e
+  | RuleElem2 C P e : C |- P e -> C |- e ∈ ORabs P
+  where "C |- P" := (valid C P)
+  .
+
+End inferRules.
+*)
+
+Definition Rel n := forall var C, relOpen var C n.
+
+Definition relV τ ξ ρ C θ : Rel 1 := fun var C => V var C τ ξ ρ C θ.
+Definition relE τ c s ρ C θ : Rel 1 := fun var C => E var C τ c s ρ C θ.
+
+Theorem sound_wrt_bound_proof : sound_wrt_bounded.
+Proof.
+  admit.
+Qed.
+
+Module ClosedPHOAS.
+
+Notation "⊤" := (Rtrue _).
+Notation "⊥" := (Rtrue _).
+(* Notation "\ e , p" := (Rabs (fun e => p)) (at level 200, format "\ e , p"). *)
+Notation "\ x .. y , p" := (Rabs (fun x => .. (Rabs (fun y => p)) ..)) (at level 200, x binder, y binder, right associativity).
+Notation "∀ x .. y , p" := (Rforalle (fun x => .. (Rforalle (fun y => p)) ..)) (at level 200, x binder, y binder, right associativity).
+Notation "∃ x .. y , p" := (Rexistse (fun x => .. (Rexistse (fun y => p)) ..)) (at level 200, x binder, y binder, right associativity).
+Notation "∀1 x .. y , p" := (Rforall1 (fun x => .. (Rforall1 (fun y => p)) ..)) (at level 200, x binder, y binder, right associativity).
+Notation "∃1 x .. y , p" := (Rexists1 (fun x => .. (Rexists1 (fun y => p)) ..)) (at level 200, x binder, y binder, right associativity).
+Definition RforallR' var n P := (@RforallR var n (fun x => P (Rvar _ _ x))).
+Notation "∀2 x .. y , p" := (RforallR' (fun x => .. (RforallR' (fun y => p)) ..)) (at level 200, x binder, y binder, right associativity).
+Definition RexistsR' var n P := (@RexistsR var n (fun x => P (Rvar _ _ x))).
+Notation "∃2 x .. y , p" := (RexistsR' (fun x => .. (RexistsR' (fun y => p)) ..)) (at level 200, x binder, y binder, right associativity).
+Definition Rrecur' var n P := (@Rrecur var n (fun x => P (Rvar _ _ x))).
+Notation "@ x .. y , p" := (Rrecur' (fun x => .. (Rrecur' (fun y => p)) ..)) (at level 200, x binder, y binder, right associativity).
+Notation "⌈ P ⌉" := (Rinj _ P).
+Notation "e ∈ P" := (Rapp P e) (at level 70).
+Infix "/\" := Rand.
+Infix "\/" := Ror.
+Infix "⇒" := Rimply (at level 90).
+Notation "▹" := Rlater.
+Definition VSet var τ (S : rel var 1) := ∀ v, v ∈ S ⇒ ⌈v ↓ τ⌉.
+
+Section TestNotations.
+  
+  Variable var : nat -> Type.
+
+  Definition ttt1 : rel var 1 := \e , ⊤.
+  Definition ttt2 : rel var 1 := \e , ⌈e ↓ Tunit⌉.
+  Definition ttt3 : rel var 1 := \_ , ⌈True /\ True⌉.
+
+End TestNotations.
+
+Inductive thresholds :=
+| THleaf
+| THarrow : thresholds -> csize -> thresholds -> thresholds
+.
+
+(* A "step-indexed" kriple model *)
+
+(* the logical relation *)
+Section LR.
+  
+  Variable var : nat -> Type.
+
+  Definition substs : Type.
+    admit.
+  Defined.
+
+  Definition substs_type : substs -> type -> type.
+    admit.
+  Defined.
+
+  Coercion substs_type : substs >-> Funclass.
+
+  Definition substs_sem : substs -> nat -> rel var 1.
+    admit.
+  Defined.
+
+  Instance Apply_substs_nat_rel : Apply substs nat (rel var 1) :=
     {
       apply := substs_sem
     }.
@@ -537,143 +754,44 @@ Section LR.
       add := add_csize
     }.
 
-  Definition add_pair : (type * relOpen var C 1) -> substs -> substs.
+  Definition add_pair : (type * rel var 1) -> substs -> substs.
     admit.
   Defined.
 
-  Instance Add_pair_substs : Add (type * relOpen var C 1) substs substs :=
+  Instance Add_pair_substs : Add (type * rel var 1) substs substs :=
     {
       add := add_pair
     }.
 
-  Definition E' V τ (c : cexpr) (s : size) (ρ : substs) Ct (θ : thresholds) : relOpen var C 1 :=
-    \e, ∀ v, ∀1 n, ⌈|~ [] e (ρ τ) /\ ⇓ e n v⌉ ⇒ ⌈ ⌊ ñ | n ≤ Ct * ñ ⌋ (ρ $ c) ⌉ /\ ∃1 ξ : csize, ⌈ξ ≤ ρ $$ s⌉ /\ v ∈ V τ ξ ρ Ct θ.
+  Program Fixpoint E' V τ (n : nat) (s : size) (ρ : substs) (C : nat) (θ : thresholds) {measure n} : rel var 1 :=
+    \e, ⌈|~ [] e (ρ τ)⌉ /\ 
+        ∀1 n', ∀ e', 
+          (⌈nstepsex e n' 0 e'⌉ ⇒ ⌈n' ≤ n⌉ /\ (⌈IsValue e'⌉ ⇒ e' ∈ V ρ C θ /\ ⌈|e'| ≤ s⌉)) /\
+          match n with
+            | 0 => ⊤
+            | S _ =>
+              (⌈nstepsex e (S n') 1 e'⌉ ⇒ ⌈(S n') ≤ n⌉ /\ ▹ (e' ∈ E' V τ (n - S n') s ρ C θ))
+          end.
+  Next Obligation.
+    omega.
+  Defined.
 
-  Fixpoint V τ (ξ : csize) (ρ : substs) (Ct : nat) (θ : thresholds) {struct τ} : relOpen var C 1 :=
-    match τ, ξ, θ with
-      | Tvar α, _, _ => ρ $ α
-      | Tunit, _, _ => \v, ⌈v ↓ τ⌉
-      | τ₁ × τ₂, CSpair ξ₁ ξ₂, _ => \v, ⌈v ↓ ρ τ⌉ /\ ∃ a b, ⌈v = Epair a b⌉ /\ a ∈ V τ₁ ξ₁ ρ Ct θ /\ b ∈ V τ₂ ξ₂ ρ Ct θ
-      | τ₁ + τ₂, CSinl ξ, _ => \v, ⌈v ↓ ρ τ⌉ /\ ∃ v', ⌈v = Einl τ₂ v'⌉ /\ v' ∈ V τ₁ ξ ρ Ct θ
-      | τ₁ + τ₂, CSinr ξ, _ => \v, ⌈v ↓ ρ τ⌉ /\ ∃ v', ⌈v = Einr τ₁ v'⌉ /\ v' ∈ V τ₂ ξ ρ Ct θ
-      | Tarrow τ₁ c s τ₂, _, THarrow θ₁ ξ₀ θ₂ => \v, ⌈v ↓ ρ τ⌉ /\ ∀1 ξ₁, ∀ v₁, v₁ ∈ V τ₁ ξ₁ ρ Ct θ /\ ⌈ξ₀ ≤ |v₁|⌉ ⇒ Eapp v v₁ ∈ E' V τ₂ c s (add ξ₁ ρ) Ct θ₂
-      | Tuniversal c s τ, _, _ => \v, ⌈v ↓ ρ τ⌉ /\ ∀1 τ', ∀2 S, VSet τ' S ⇒ Etapp v τ' ∈ E' V τ c s (add (τ', S) ρ) Ct θ
-      | Trecur τ, CSfold ξ, _ => @S, \v, ⌈v ↓ ρ τ⌉ /\ ∃ v', ⌈v = Efold τ v'⌉ /\ ▹ (v' ∈ V τ ξ (add (ρ τ, S) ρ) Ct θ)
-      | _, _, _ => \_, ⊥
+  Fixpoint V τ (ρ : substs) (C : nat) (θ : thresholds) {struct τ} : rel var 1 :=
+    match τ, θ with
+      | Tvar α, _ => ρ $ α
+      | Tunit, _ => \v, ⌈v ↓ τ⌉
+      | τ₁ × τ₂, _ => \v, ⌈v ↓ ρ τ⌉ /\ ∃ a b, ⌈v = Epair a b⌉ /\ a ∈ V τ₁ ρ C θ /\ b ∈ V τ₂ ρ C θ
+      | τ₁ + τ₂, _ => \v, ⌈v ↓ ρ τ⌉ /\ ∃ v', (⌈v = Einl τ₂ v'⌉ /\ v' ∈ V τ₁ ρ C θ) /\ ⌈v = Einr τ₁ v'⌉ /\ v' ∈ V τ₂ ρ C θ
+      | Tarrow τ₁ c s τ₂, THarrow θ₁ ξ₀ θ₂ => \v, ⌈v ↓ ρ τ⌉ /\ ∀ v₁, v₁ ∈ V τ₁ ρ C θ ⇒ Eapp v v₁ ∈ E' (V τ₂) τ₂ (cexpr_to_nat c) s (add (if ξ₀ <=? |v₁| then |v₁| else ξ₀) ρ) C θ₂
+      | Tuniversal c s τ, _ => \v, ⌈v ↓ ρ τ⌉ /\ ∀1 τ', ∀2 S, VSet τ' S ⇒ Etapp v τ' ∈ E' (V τ) τ (cexpr_to_nat c) s (add (τ', S) ρ) C θ
+      | Trecur τ, _ => @S, \v, ⌈v ↓ ρ τ⌉ /\ ∃ v', ⌈v = Efold τ v'⌉ /\ ▹ (v' ∈ V τ (add (ρ τ, S) ρ) C θ)
+      | _, _ => \_, ⊥
     end
   .
 
-  Definition E := E' V.
+  Definition E τ := E' (V τ).
 
 End LR.
 
-End OpenPHOAS.
-
-Import OpenPHOAS.
-
-Definition valid (X : list bool) {var} C (ctxP : list (relOpen var C 0)) (P : relOpen var C 0) : Prop.
-  admit.
-Defined.
-Notation "|- X C ctxP P" := (valid X C ctxP P) (at level 90).
-
-Definition add_var t ctx Ps ρ :=
-  let ctx := t :: ctx in 
-  let Ps := lift t Ps in
-  let ρ := lift t ρ in
-  (ctx, Ps, ρ).
-
-Definition add_type k :=
-  let Pack ctx0 Ps ρ := C in
-  let (ctx, Ps, ρ) := add_var TTtype ctx0 Ps ρ in
-  let Ps := extend ctx0 (fun τ => kinding [] τ k) :: Ps in
-  match k with
-    | KDstar => 
-      let (ctx, Ps, ρ) := add_var (TTrel 1) ctx Ps ρ in
-      let Ps := extend ctx0 (fun τ S => VSet τ S) :: Ps in
-      let ρ := SEtype #1 (Some #0) :: ρ in
-      Pack ctx Ps ρ
-    | _ =>
-      let ρ := SEtype #1 None :: ρ in
-      Pack ctx Ps ρ
-  end.
-
-Definition add_expr τ θ os :=
-  let Pack ctx0 Ps ρ := C in
-  let (ctx, Ps, ρ) := add_var TTexpr ctx0 Ps ρ in
-  let Ps := #0 ∈ V τ ρ Ct θ :: Ps in
-  let (ctx, Ps, ρ) := add_var (TTother csize) ctx0 Ps ρ in
-  let ρ := SEexpr #1 #0 :: ρ in
-  match os with
-    | inl ξ₀ =>
-      let Ps := extend ctx0 (fun v ξ => ξ₀ ≤ |v| ? ξ = |v| : ξ = ξ₀) C :: Ps in
-      Pack ctx Ps ρ
-    | inr s =>
-      let Ps := extend (TTexpr :: ctx0) (fun ξ => asCsize (fun ξs => ξ = ξs) (ρ $$ s)) in
-      Pack ctx Ps ρ
-  end.
-
-Fixpoint makeC Γ :=
-  match Γ with
-    | nil => (nil, nil)
-    | e : Γ =>
-      let C := makeC Γ in
-      match e with
-        | TEkinging k =>
-          add_type k C
-        | TEtyping (τ, θ, os) =>
-          add_expr τ θ os C
-      end
-  end.
-
-Definition related Γ e τ c s :=
-  exists C ξs θs θ Γ',
-    extendΓ Γ ξs θs = Some Γ' /\
-    let (C, ρ) := makeC Γ' in
-    C |- (ρ $ e) ∈ E τ (C * c) s ρ C θ
-    (* ⊢ Γ e τ c s /\ *)
-    let X := map () Γ in
-    let C := map () Γ in
-    let ρ := map () Γ in
-    let ctxP := map () Γ in
-    |- X C ctxP (e ∈ E c s ρ C θ)
-      
-(*
-Section inferRules.
-
-  Variable var : nat -> Type.
-
-  Variable C : list nat.
-
-  Reserved Notation "C |- P" (at level 90).
-  
-  Inductive valid : list (relOpen var C 0) -> relOpen var C 0 -> Prop :=
-  | RuleMono C P : C |- P -> C |- ▹P
-  | RuleLob C P : ▹P :: C |- P -> C |- P
-  | RuleLaterAnd1 C P Q : C |- ▹ (P /\ Q) -> C |- ▹P /\ ▹Q
-  | RuleLaterAnd2 C P Q : C |- ▹P /\ ▹Q -> C |- ▹ (P /\ Q)
-  | RuleElem1 C P e : C |- e ∈ ORabs P -> C |- P e
-  | RuleElem2 C P e : C |- P e -> C |- e ∈ ORabs P
-  where "C |- P" := (valid C P)
-  .
-
-End inferRules.
-*)
-
-Definition Rel n := forall var C, relOpen var C n.
-
-Definition relV τ ξ ρ C θ : Rel 1 := fun var C => V var C τ ξ ρ C θ.
-Definition relE τ c s ρ C θ : Rel 1 := fun var C => E var C τ c s ρ C θ.
-
-Lemma foundamental :
-  forall Γ e τ c s,
-    ⊢ Γ e τ c s -> 
-    ⊩ Γ e τ c s.
-Proof.
-  admit.
-Qed.
-
-Theorem sound_wrt_bound_proof : sound_wrt_bounded.
-Proof.
-  admit.
-Qed.
+End ClosedPHOAS.
 
